mid-attempt to tweak splitp semantics, starting skeleton of full system proofs

src/Impl_vm.v
@@ -6,8 +6,18 @@ Author:  Adam Petz, ampetz@ku.edu
 
 Require Import Term_Defs Term GenStMonad MonadVM.
 
+Require Import List.
+Import ListNotations.
+
 (** Monadic VM implementation *)
 
+
+(*
+Fixpoint copland_compile (t:AnnoTerm): CVM (list (CVM unit)) :=
+  ret [].
+*)
+
+  
 Fixpoint copland_compile (t:AnnoTerm): CVM unit :=
   match t with
   | aasp (n,_) _ a =>
@@ -33,10 +43,25 @@ Fixpoint copland_compile (t:AnnoTerm): CVM unit :=
       copland_compile t2 ;;
       e2r <- get_ev ;;
       join_seq (Nat.pred y) p e1r e2r
-  | abpar (x,y) _ (loc_e1,loc_e1') (loc_e2,loc_e2') (sp1,sp2) t1 t2 =>
+  | abpar (x,y) _ (*(loc_e1,loc_e1')*) (loc_e2,loc_e2') (sp1,sp2) t1 t2 =>
       e <- get_ev ;;
       p <- get_pl ;;
-      split_ev_par x sp1 sp2 loc_e1 loc_e2 t1 t2 e p ;;
+      e1 <- split_ev_par x sp1 sp2 (*loc_e1*) loc_e2 (*t1 t2*) e p ;;
+      put_ev e1 ;;
+      copland_compile t1 ;;
+      e1r <- get_ev ;;
+
+      e2 <- get_store_at loc_e2 ;;
+      put_ev e2 ;;
+      copland_compile t2 ;;
+      e2r_store <- get_ev ;;
+      put_store_at loc_e2' e2r_store ;;
+
+      (*
+      runParThread t2 p loc_e2 loc_e2' *)
+
+
+      
       (*let '(loc_e1,loc_e2) := pr in*)
       (*let loc_e1 := fst (range t1) in *)
 
@@ -56,14 +81,104 @@ Fixpoint copland_compile (t:AnnoTerm): CVM unit :=
       put_store_at loc_e1 e1 ;;
       put_store_at loc_e2 e2 ;;
        *)
-      
-      runParThreads t1 t2 p loc_e1 loc_e1' loc_e2 loc_e2'  ;;
-      join_par (Nat.pred y) p loc_e1' loc_e2'
+
+
+      (*
+      runParThreads t1 t2 p loc_e1 loc_e1' loc_e2 loc_e2'  ;; *)
+      join_par (Nat.pred y) p (*loc_e1'*) e1r loc_e2'
       (*
       e1r <- get_store_at loc_e1' ;;
       e2r <- get_store_at loc_e2' ;;
       join_par (Nat.pred y) p e1r e2r *)
   end.
+
+Require Import Maps.
+
+Definition setup := MapC Plc (CVM unit).
+
+(*
+Require Import OptMonad. *)
+
+Definition add_at (s:setup) (q:Plc) (comp:CVM unit) : setup :=
+  let old_comp := map_get s q in
+  match old_comp with
+  | Some m =>
+      let new_comp := m ;; comp in
+      map_set s q new_comp
+  | _ => map_set s q comp
+  end.
+
+Definition bookend (comp: CVM unit) (req_loc rpy_loc:Loc): CVM unit :=
+  e <- get_store_at req_loc ;;
+  put_ev e ;;
+  comp ;;
+  e' <- get_ev ;;
+  put_store_at rpy_loc e'.
+
+Fixpoint copland_compliment (t:AnnoTerm) (s:setup): setup :=
+  match t with
+  | aatt (i,j) _ (req_loc,rpy_loc) q t' =>
+    let comp := copland_compile t' in (* TODO: annotate terms with the place they execute? *)
+    add_at s q (bookend comp req_loc rpy_loc)
+  | alseq r _ t1 t2 =>
+    let s1 := copland_compliment t1 s in
+    let s2 := copland_compliment t2 s1 in
+    s2
+  | _ => []
+  end.
+
+Require Import EqClass.
+
+Fixpoint map_vals{A B:Type} `{H : EqClass A} (m : MapC A B ) : list B :=
+  match m with
+  | [] => []
+  | (k', v) :: m' => v :: map_vals m'
+  end.
+
+(*
+Definition add_before (s:setup) (q:Plc) (comp:CVM unit) : setup :=
+  let old_comp := map_get s q in
+  match old_comp with
+  | Some m =>
+      let new_comp := comp ;; m in
+      map_set s q new_comp
+  | _ => map_set s q comp
+  end.
+*)
+    
+
+Definition orchestrate (t:AnnoTerm): ((CVM unit) * setup) :=
+  let main_thread := copland_compile t in
+  let servers := copland_compliment t map_empty in
+  (main_thread, servers).
+  
+
+Record PlatformState : Type := mk_plat
+                         {plat_pl:Plc ;
+                          plat_trace:list Ev ;
+                          plat_store:ev_store}.
+
+Definition start (st:PlatformState) (places:(CVM unit) * setup) : PlatformState.
+Admitted.
+
+Definition run_it (me:Plc) (t:AnnoTerm) : PlatformState :=
+  start (mk_plat me [] []) (orchestrate t).
+
+Definition getLocs (t:Term) (m:MapC (Plc*Plc) (list Loc)): list Loc.
+Admitted.
+
+Definition fromSome{A:Type} (default:A) (opt:option A): A :=
+  match opt with
+  | Some x => x
+  | _ => default
+  end.
+
+Definition run_it_term (me:Plc) (t:Term) (m:MapC (Plc*Plc) (list Loc)) : PlatformState :=
+  let annt := snd (anno' t 0 (getLocs t m)) in
+  run_it me annt.
+
+
+
 
 Definition run_cvm (t:AnnoTerm) st : cvm_st :=
   execSt (copland_compile t) st.
