src/Auto.v
@@ -83,13 +83,15 @@ Ltac jkjk' :=
   | H: _ |- _ => rewrite H; reflexivity
   end.
 
-Lemma hhh : forall t1 t2 a b c d r lr s,
-    well_formed (abpar r lr (a,b) (c,d) s t1 t2) -> 
+(*
+Lemma hhh : forall t1 t2 (*a b*) c d r lr s,
+    well_formed (abpar r lr (*(a,b)*) (c,d) s t1 t2) -> 
     (*range t1 = (a,b) ->
     range t2 = (c,d) -> *)
     PeanoNat.Nat.eqb a c = false.
 Proof.
 Admitted.
+*)
 
 
 (*
@@ -128,7 +130,7 @@ Proof.
 Defined.
  *)
 
-
+(*
 Lemma hhhh : forall t1 t2 a b c d r lr s,
     well_formed (abpar r lr (a,b) (c,d) s t1 t2) ->
     (*range t1 = (a,b) ->
@@ -136,6 +138,7 @@ Lemma hhhh : forall t1 t2 a b c d r lr s,
     PeanoNat.Nat.eqb c b (*(b - 1)*) = false.
 Proof.
 Admitted.
+*)
 
 (*
 
@@ -273,6 +276,7 @@ Proof.
 Defined.
  *)
 
+(*
 Lemma hhhhh : forall t1 t2 a b c d r lr s,
     well_formed (abpar r lr (a,b) (c,d) s t1 t2) ->
     (*range t1 = (a,b) ->
@@ -280,6 +284,7 @@ Lemma hhhhh : forall t1 t2 a b c d r lr s,
     PeanoNat.Nat.eqb b d (* (b - 1) (d - 1) *) = false.
 Proof.
 Admitted.
+*)
 
 
 
@@ -357,6 +362,7 @@ Proof.
 Defined.
 *)
 
+(*
 Lemma abpar_store_non_overlap : forall t1 t2 a b c d r lr s,
     well_formed (abpar r lr (a,b) (c,d) s t1 t2) ->
     (*range t1 = (a,b) ->
@@ -371,6 +377,23 @@ Proof.
   eapply hhhh; eauto.
   eapply hhhhh; eauto.
 Defined.
+ *)
+
+Lemma abpar_store_non_overlap : forall t1 t2 (*a b *) c d r lr s,
+    well_formed (abpar r lr (*(a,b)*) (c,d) s t1 t2) ->
+    PeanoNat.Nat.eqb c d = false.
+    (*
+    (*range t1 = (a,b) ->
+    range t2 = (c,d) -> *)
+    PeanoNat.Nat.eqb a c = false /\
+    PeanoNat.Nat.eqb c b (* (b - 1) *) = false /\
+    PeanoNat.Nat.eqb b d (* (b - 1) (d - 1) *) = false.
+     *)
+Proof.
+Admitted.
+
+
+
 
 Ltac fail_no_match :=
   match goal with
@@ -389,13 +412,19 @@ Ltac fail_no_match_some :=
 Ltac htac'' :=
   (*let tac := eapply h''; eauto in *)
   match goal with
-  | [H: well_formed (abpar _ _ (?a,?b) (?c,?d) _ ?t1 ?t2) (*,
+  | [H: well_formed (abpar _ _ (*(?a,?b)*) (?c,?d) _ ?t1 ?t2) (*,
         H2: range ?t1 = (?a,?b),
             H3: range ?t2 = (?c,?d) *) |- _] =>
     let W := fresh in
-    let X := fresh in
+    assert (PeanoNat.Nat.eqb c d = false) as W
+        by (eapply abpar_store_non_overlap; apply H);
+    try (rewrite W in *; clear W)
+  end.
+    (* let X := fresh in
     let Y := fresh in
-    let Z := fresh in
+    let Z := fresh in *)
+
+    (*
     assert (PeanoNat.Nat.eqb a c = false /\
             PeanoNat.Nat.eqb c b (* (b - 1) *) = false /\
             PeanoNat.Nat.eqb b d (* (b - 1) (d - 1) *) = false) as W
@@ -405,8 +434,11 @@ Ltac htac'' :=
     try (rewrite Y in *; clear Y);
     try (rewrite Z in *; clear Z)
   end.
+*)
 
 Ltac dohtac := fail_no_match_some;
-               try htac'';
+               (*try htac''; *)
                try rewrite PeanoNat.Nat.eqb_refl in *;
                try rewrite PeanoNat.Nat.eqb_eq in *.
+
+(* hi *)
